boogie/scheduler-queue/bst-delete-inside.bpl
@@ -1,0 +1,439 @@
+// Supporting Artifact for
+// "Predictive Verification using Intrinsic Definitions of Data Structures"
+// by Adithya Murali, Cody Rivera, and P. Madhusudan.
+// 
+// Artifact by Cody Rivera, 2023. 
+//
+// Verification of deleting inside a BST, for overlaid data structures.
+
+procedure BSTFixDepthContract(q1s: Ref, q1t: Ref, x: Ref);
+    requires x != null;
+    requires RefSetsDisjoint(
+        (C.bst_repr[x])[x := false],
+        Br_bst
+    );
+    requires RefSetsEqual(Br_list, EmptyRefSet);
+    requires LC_Trans_NoDepth(C.k, C.l, C.r, C.p, C.min, C.max, C.bst_size,
+                C.bst_keys, C.bst_repr, C.bst_depth, C.bst_root,
+                C.next, C.prev, C.list_keys, C.list_repr, x);
+    requires C.p[x] != null;
+    modifies Br_bst, Br_list, C.bst_depth;
+    ensures LC(C.k, C.l, C.r, C.p, C.min, C.max, C.bst_size,
+                C.bst_keys, C.bst_repr, C.bst_depth, C.bst_root,
+                C.next, C.prev, C.list_keys, C.list_repr, x);
+    ensures RefSetsEqual(Br_bst, old(Br_bst)[x := false]);
+    ensures RefSetsEqual(Br_list, EmptyRefSet);
+    // Framing conditions
+    ensures Frame_all(
+        C.k, C.l, C.r, C.p, C.min, C.max, C.bst_size,
+        C.bst_keys, C.bst_repr, C.bst_depth, C.bst_root,
+        C.next, C.prev, C.list_keys, C.list_repr,
+        old(C.k), old(C.l), old(C.r), old(C.p), old(C.min), old(C.max), old(C.bst_size),
+        old(C.bst_keys), old(C.bst_repr), old(C.bst_depth), old(C.bst_root),
+        old(C.next), old(C.prev), old(C.list_keys), old(C.list_repr),
+        RefSetIntersectF(old(C.bst_repr)[x], old(C.bst_repr)[old(C.bst_root)[x]]), old(alloc)
+    );
+
+procedure BSTRemoveRootInsideContract(q1s: Ref, q1t: Ref, x: Ref)
+    returns (ret: Ref, root: Ref);
+    requires x != null;
+    requires RefSetsDisjoint(
+        C.bst_repr[x],
+        Br_bst
+    );
+    requires RefSetsEqual(Br_list, EmptyRefSet);
+    requires LC(C.k, C.l, C.r, C.p, C.min, C.max, C.bst_size,
+                C.bst_keys, C.bst_repr, C.bst_depth, C.bst_root,
+                C.next, C.prev, C.list_keys, C.list_repr, x);
+    requires C.p[x] != null;
+    requires C.l[C.p[x]] == x || C.r[C.p[x]] == x;
+    requires !(C.l[C.p[x]] == x && C.r[C.p[x]] == x);
+    requires C.next[x] == null && C.prev[x] == null;
+    requires q1s != null ==> x != q1s;
+    modifies Br_bst, Br_list, C.l, C.r, C.p, C.min, C.max, C.bst_size,
+                C.bst_keys, C.bst_repr, C.bst_depth, C.bst_root;
+    ensures root != null;
+    ensures ret == null || ret == old(C.l)[x] || ret == old(C.r)[x];
+    ensures (RefSetsEqual(old(C.bst_repr)[x], EmptyRefSet[x := true]) ==> ret == null);
+    ensures ((RefSetSubset(EmptyRefSet[x := true], old(C.bst_repr)[x]) 
+             && !RefSetsEqual(old(C.bst_repr)[x], EmptyRefSet[x := true]))
+                ==> ret != null);
+    ensures (ret != null ==>
+                LC(C.k, C.l, C.r, C.p, C.min, C.max, C.bst_size,
+                    C.bst_keys, C.bst_repr, C.bst_depth, C.bst_root,
+                    C.next, C.prev, C.list_keys, C.list_repr, ret)
+                && KeySetsEqual(C.bst_keys[ret], (old(C.bst_keys)[x])[C.k[x] := false])
+                && C.min[ret] >= old(C.min)[x]
+                && C.max[ret] <= old(C.max)[x]
+                && RefSetsEqual(C.bst_repr[ret], (old(C.bst_repr)[x])[x := false])
+                && C.bst_root[ret] == old(C.bst_root)[x]
+                && C.p[ret] == old(C.p)[x]
+                // && listfieldsunchanged(ret)
+                );
+    ensures old(C.l)[old(C.p)[x]] == x ==> C.l[old(C.p)[x]] == ret;
+    ensures old(C.l)[old(C.p)[x]] != x ==> C.l[old(C.p)[x]] == old(C.l)[old(C.p)[x]];
+    ensures old(C.r)[old(C.p)[x]] == x ==> C.r[old(C.p)[x]] == ret;
+    ensures old(C.r)[old(C.p)[x]] != x ==> C.r[old(C.p)[x]] == old(C.r)[old(C.p)[x]];
+    ensures old(C.k)[old(C.p)[x]] == C.k[old(C.p)[x]];
+    ensures old(C.p)[old(C.p)[x]] == C.p[old(C.p)[x]];
+    ensures old(C.bst_size)[old(C.p)[x]] == C.bst_size[old(C.p)[x]];
+    ensures KeySetsEqual(old(C.bst_keys)[old(C.p)[x]], C.bst_keys[old(C.p)[x]]);
+    ensures RefSetsEqual(old(C.bst_repr)[old(C.p)[x]], C.bst_repr[old(C.p)[x]]);
+    ensures old(C.min)[old(C.p)[x]] == C.min[old(C.p)[x]];
+    ensures old(C.max)[old(C.p)[x]] == C.max[old(C.p)[x]];
+    ensures old(C.bst_depth)[old(C.p)[x]] == C.bst_depth[old(C.p)[x]];
+    ensures old(C.bst_root)[old(C.p)[x]] == C.bst_root[old(C.p)[x]];
+    // ensures listfieldsunchanged(old(x.p));
+    ensures root == x && C.k[root] == old(C.k)[x];
+    ensures LC(C.k, C.l, C.r, C.p, C.min, C.max, C.bst_size,
+                C.bst_keys, C.bst_repr, C.bst_depth, C.bst_root,
+                C.next, C.prev, C.list_keys, C.list_repr, root);
+    ensures BST_Isolated(C.k, C.l, C.r, C.p, C.min, C.max, C.bst_size,
+                C.bst_keys, C.bst_repr, C.bst_depth, C.bst_root,
+                C.next, C.prev, C.list_keys, C.list_repr, root);
+    // ensures listfieldsunchanged(root);
+    ensures q1s != null ==> C.bst_root[q1s] == old(C.bst_root)[q1s];
+    ensures old(C.p)[x] == null ==> RefSetsEqual(Br_bst, old(Br_bst));
+    ensures old(C.p)[x] != null ==> RefSetsEqual(Br_bst, old(Br_bst)[old(C.p)[x] := true]);
+    ensures RefSetsEqual(Br_list, EmptyRefSet);
+    // Framing conditions
+    ensures Frame_all(
+        C.k, C.l, C.r, C.p, C.min, C.max, C.bst_size,
+        C.bst_keys, C.bst_repr, C.bst_depth, C.bst_root,
+        C.next, C.prev, C.list_keys, C.list_repr,
+        old(C.k), old(C.l), old(C.r), old(C.p), old(C.min), old(C.max), old(C.bst_size),
+        old(C.bst_keys), old(C.bst_repr), old(C.bst_depth), old(C.bst_root),
+        old(C.next), old(C.prev), old(C.list_keys), old(C.list_repr),
+        RefSetIntersectF(old(C.bst_repr)[x], old(C.bst_repr)[old(C.bst_root)[x]])[old(C.p)[x] := true],
+        old(alloc)
+    );
+
+function {:inline} LC_BST_Trans_PlusNode_Debug(
+    k: [Ref]int, 
+    l: [Ref]Ref,
+    r: [Ref]Ref,
+    p: [Ref]Ref,
+    min: [Ref]int,
+    max: [Ref]int,
+    bst_size: [Ref]int,
+    bst_keys: [Ref]KeySet,
+    bst_repr: [Ref]RefSet,
+    bst_depth: [Ref]int,
+    bst_root: [Ref]Ref,
+    next: [Ref]Ref,
+    prev: [Ref]Ref,
+    list_keys: [Ref]KeySet,
+    list_repr: [Ref]RefSet,
+    x: Ref,
+    node: Ref
+) returns (bool)
+{
+    (x != null && node != null) ==> (
+        (x == bst_root[x] ==> 
+            (bst_repr[x])[x]
+            && p[x] == null
+            && bst_depth[x] == 0
+            && l[x] == null
+            && (r[x] == null ==>
+                    RefSetsEqual(bst_repr[x], (EmptyRefSet[x := true])[node := true])
+                    && KeySetsEqual(bst_keys[x], EmptyKeySet[k[node] := true]))
+            && (r[x] != null ==>
+                    p[r[x]] == x
+                    && RefSetsEqual(bst_repr[x], ((bst_repr[r[x]])[x := true])[node := true])
+                    && !(bst_repr[r[x]])[x]
+                    && KeySetsEqual(bst_keys[x], (bst_keys[r[x]])[k[node] := true])))
+        && (x != bst_root[x] ==>
+                (bst_repr[x])[x]
+                && min[x] <= k[x]
+                && k[x] <= max[x]
+                && p[x] != null
+                && !(bst_repr[x])[p[x]]
+                && (l[p[x]] == x || r[p[x]] == x)
+                && !(bst_repr[x])[bst_root[x]]
+                && bst_depth[x] == bst_depth[p[x]] + 1
+                && (l[x] != null ==> 
+                        (bst_repr[x])[l[x]]
+                        && !(bst_repr[l[x]])[x]
+                        && p[l[x]] == x
+                        && max[l[x]] < k[x])
+                && (r[x] != null ==> 
+                        (bst_repr[x])[r[x]]
+                        && !(bst_repr[r[x]])[x]
+                        && p[r[x]] == x
+                        && min[r[x]] > k[x])
+                && (l[x] == null && r[x] == null ==>
+                        RefSetsEqual(bst_repr[x], (EmptyRefSet[x := true])[node := true])
+                        && KeySetsEqual(bst_keys[x], (EmptyKeySet[k[x] := true])[k[node] := true])
+                        //&& min[x] == k[x] 
+                        //&& k[x] == max[x]
+                        )
+                && (l[x] != null && r[x] == null ==>
+                        RefSetsEqual(bst_repr[x], ((bst_repr[l[x]])[x := true])[node := true])
+                        && KeySetsEqual(bst_keys[x], ((bst_keys[l[x]])[k[x] := true])[k[node] := true])
+                        && !(bst_keys[l[x]])[k[x]]
+                        //&& min[x] == min[l[x]] && max[x] == k[x]
+                        )
+                && (l[x] == null && r[x] != null ==>
+                        RefSetsEqual(bst_repr[x], ((bst_repr[r[x]])[x := true])[node := true])
+                        && KeySetsEqual(bst_keys[x], ((bst_keys[r[x]])[k[x] := true])[k[node] := true])
+                        && !(bst_keys[r[x]])[k[x]]
+                        //&& min[x] == k[x] && max[x] == max[r[x]]
+                        )
+                && (l[x] != null && r[x] != null ==>
+                        RefSetsEqual(bst_repr[x], (RefSetUnionF((bst_repr[l[x]])[x := true], bst_repr[r[x]]))[node := true])
+                        && RefSetsDisjoint(bst_repr[l[x]], bst_repr[r[x]])
+                        && KeySetsEqual(bst_keys[x], (KeySetUnionF((bst_keys[l[x]])[k[x] := true], bst_keys[r[x]]))[k[node] := true])
+                        && KeySetsDisjoint(bst_keys[l[x]], bst_keys[r[x]])
+                        && !(bst_keys[l[x]])[k[x]] && !(bst_keys[r[x]])[k[x]]
+                        //&& min[x] == min[l[x]] && max[x] == max[r[x]]
+                        )
+                && bst_root[x] == bst_root[p[x]]
+                && (bst_repr[bst_root[x]])[x]
+                && (bst_repr[bst_root[x]])[p[x]]
+                && (l[x] != null ==> (bst_repr[bst_root[x]])[l[x]])
+                && (r[x] != null ==> (bst_repr[bst_root[x]])[r[x]])
+                && p[bst_root[x]] == null)
+            && bst_depth[x] >= 0
+            && (p[x] != null ==> bst_depth[p[x]] >= 0)
+            && bst_root[x] != null
+            //&& bst_size[x] == GetBSTSize(bst_size, l[x]) + 2 + GetBSTSize(bst_size, r[x])
+            && bst_size[x] >= 1
+        )
+}
+
+procedure BSTDeleteInside(q1s: Ref, q1t: Ref, root: Ref, x: Ref)
+    returns (ret: Ref, node: Ref)
+    requires root != null && x != null;
+    requires RefSetsEqual(Br_bst, EmptyRefSet);
+    requires RefSetsEqual(Br_list, EmptyRefSet);
+    requires LC(C.k, C.l, C.r, C.p, C.min, C.max, C.bst_size,
+                C.bst_keys, C.bst_repr, C.bst_depth, C.bst_root,
+                C.next, C.prev, C.list_keys, C.list_repr, x);
+    requires C.p[x] != null;
+    requires C.l[C.p[x]] == x || C.r[C.p[x]] == x;
+    requires !(C.l[C.p[x]] == x && C.r[C.p[x]] == x);
+    requires C.bst_root[x] == root;
+    requires C.next[x] == null && C.prev[x] == null;
+    requires q1s != null ==> x != q1s;
+    modifies Br_bst, Br_list, C.l, C.r, C.p, C.min, C.max, C.bst_size,
+                C.bst_keys, C.bst_repr, C.bst_depth, C.bst_root;
+    ensures node != null;
+    ensures ret == null || ret == old(C.l)[x] || ret == old(C.r)[x];
+    ensures (RefSetsEqual(old(C.bst_repr)[x], EmptyRefSet[x := true]) ==> ret == null);
+    ensures ((RefSetSubset(EmptyRefSet[x := true], old(C.bst_repr)[x]) 
+             && !RefSetsEqual(old(C.bst_repr)[x], EmptyRefSet[x := true]))
+                ==> ret != null);
+    ensures (ret != null ==>
+                LC(C.k, C.l, C.r, C.p, C.min, C.max, C.bst_size,
+                    C.bst_keys, C.bst_repr, C.bst_depth, C.bst_root,
+                    C.next, C.prev, C.list_keys, C.list_repr, ret)
+                && KeySetsEqual(C.bst_keys[ret], (old(C.bst_keys)[x])[C.k[x] := false])
+                && C.min[ret] >= old(C.min)[x]
+                && C.max[ret] <= old(C.max)[x]
+                && RefSetsEqual(C.bst_repr[ret], (old(C.bst_repr)[x])[x := false])
+                && C.bst_root[ret] == root
+                && C.p[ret] == old(C.p)[x]
+                // && listfieldsunchanged(ret)
+                );
+    ensures KeySetsEqual(C.bst_keys[root], (old(C.bst_keys)[root])[C.k[x] := false]);
+    ensures C.min[root] == old(C.min)[root];
+    ensures C.max[root] == old(C.max)[root];
+    ensures RefSetsEqual(C.bst_repr[root], (old(C.bst_repr)[root])[x := false]);
+    ensures C.bst_root[root] == old(C.bst_root)[root];
+    ensures C.p[root] == old(C.p)[root];
+    // ensures listfieldsunchanged(root);
+    ensures node == x && C.k[node] == old(C.k)[x];
+    ensures LC(C.k, C.l, C.r, C.p, C.min, C.max, C.bst_size,
+                C.bst_keys, C.bst_repr, C.bst_depth, C.bst_root,
+                C.next, C.prev, C.list_keys, C.list_repr, node);
+    ensures BST_Isolated(C.k, C.l, C.r, C.p, C.min, C.max, C.bst_size,
+                C.bst_keys, C.bst_repr, C.bst_depth, C.bst_root,
+                C.next, C.prev, C.list_keys, C.list_repr, node);
+    // ensures listfieldsunchanged(node);
+    ensures q1s != null ==> C.bst_root[q1s] == old(C.bst_root)[q1s];
+    ensures RefSetsEqual(Br_list, EmptyRefSet);
+    ensures RefSetsEqual(Br_list, EmptyRefSet);
+    // Framing conditions
+    ensures Frame_all(
+        C.k, C.l, C.r, C.p, C.min, C.max, C.bst_size,
+        C.bst_keys, C.bst_repr, C.bst_depth, C.bst_root,
+        C.next, C.prev, C.list_keys, C.list_repr,
+        old(C.k), old(C.l), old(C.r), old(C.p), old(C.min), old(C.max), old(C.bst_size),
+        old(C.bst_keys), old(C.bst_repr), old(C.bst_depth), old(C.bst_root),
+        old(C.next), old(C.prev), old(C.list_keys), old(C.list_repr),
+        old(C.bst_repr)[old(C.bst_root)[x]],
+        old(alloc)
+    );
+{
+    // Local variables
+    var p: Ref;
+    var cur: Ref;
+
+    // Subexpressions
+    var p_l: Ref; var p_r: Ref; var cur_p: Ref;
+    var cur_l: Ref; var cur_r: Ref; var cur_k: int;
+    var cur_l_bst_size: int; var cur_r_bst_size: int;
+    var cur_l_min: int; var cur_l_bst_keys: KeySet;
+    var cur_l_bst_repr: RefSet;
+    var cur_r_max: int; var cur_r_bst_keys: KeySet;
+    var cur_r_bst_repr: RefSet;
+
+    // Heap value, PreLoop0:
+    var C.k_pl0: [Ref]int;
+    var C.l_pl0: [Ref]Ref; var C.r_pl0: [Ref]Ref;
+    var C.p_pl0: [Ref]Ref; var C.min_pl0: [Ref]int; var C.max_pl0: [Ref]int;
+    var C.bst_size_pl0: [Ref]int; var C.bst_keys_pl0: [Ref]KeySet; var C.bst_repr_pl0: [Ref]RefSet;
+    var C.bst_depth_pl0: [Ref]int; var C.bst_root_pl0: [Ref]Ref;
+    var C.next_pl0: [Ref]Ref; var C.prev_pl0: [Ref]Ref;
+    var C.list_keys_pl0: [Ref]KeySet; var C.list_repr_pl0: [Ref]RefSet;
+
+    // Loop termination
+    var t: int;
+    var z: int;
+
+    call InAllocParam(q1s);
+    call InAllocParam(q1t);
+    call InAllocParam(root);
+    call InAllocParam(x);
+
+    call p := Get_p(x);
+    call IfNotBr_ThenLC(p);
+    call p_l := Get_l(p);
+    call p_r := Get_r(p);
+    if (p_l != null) {
+        call IfNotBr_ThenLC(p_l);
+    }
+    if (p_r != null) {
+        call IfNotBr_ThenLC(p_r);
+    }
+    call ret, node := BSTRemoveRootInsideContract(q1s, q1t, x);
+    cur := p;
+
+    call IfNotBrList_ThenListLC(cur);
+
+    // label PreLoop0:
+    C.k_pl0 := C.k;
+    C.l_pl0 := C.l; C.r_pl0 := C.r;
+    C.p_pl0 := C.p; C.min_pl0 := C.min; C.max_pl0 := C.max;
+    C.bst_size_pl0 := C.bst_size; C.bst_keys_pl0 := C.bst_keys; C.bst_repr_pl0 := C.bst_repr;
+    C.bst_depth_pl0 := C.bst_depth; C.bst_root_pl0 := C.bst_root;
+    C.next_pl0 := C.next; C.prev_pl0 := C.prev;
+    C.list_repr_pl0 := C.list_repr; C.list_keys_pl0 := C.list_keys;
+
+    // Since this is a ghost loop, we must prove termination of it
+    call cur_p := Get_p(cur);
+
+    while (cur_p != null)
+        invariant cur != null;
+        invariant cur_p == C.p[cur];
+        invariant RefSetsEqual(Br_bst, EmptyRefSet[cur := true]);
+        invariant RefSetsEqual(Br_list, EmptyRefSet);
+        invariant LC_Trans_PlusNode(C.k, C.l, C.r, C.p, C.min, C.max, C.bst_size,
+                C.bst_keys, C.bst_repr, C.bst_depth, C.bst_root,
+                C.next, C.prev, C.list_keys, C.list_repr, cur, node);
+        invariant (C.bst_keys[cur])[C.k[node]];
+        invariant C.p[cur] != null && C.l[cur] != null ==> (
+            !(C.bst_repr[C.l[cur]])[node]
+            && !(C.bst_keys[C.l[cur]])[C.k[node]]
+            && C.min[cur] <= C.min[C.l[cur]]
+            && C.max[C.l[cur]] < C.k[cur]
+        );
+        invariant C.p[cur] != null && C.r[cur] != null ==> (
+            !(C.bst_repr[C.r[cur]])[node]
+            && !(C.bst_keys[C.r[cur]])[C.k[node]]
+            && C.k[cur] < C.min[C.r[cur]]
+            && C.max[C.r[cur]] <= C.max[cur]
+        );
+        invariant (C.bst_repr[root])[cur];
+        invariant C.bst_root[cur] == root;
+        invariant C.p[cur] != null ==> C.k[cur] != C.k[node];
+        invariant Unchanged(
+            C.k, C.l, C.r, C.p, C.min, C.max, C.bst_size,
+            C.bst_keys, C.bst_repr, C.bst_depth, C.bst_root,
+            C.next, C.prev, C.list_keys, C.list_repr,
+            C.k_pl0, C.l_pl0, C.r_pl0, C.p_pl0, C.min_pl0, C.max_pl0, C.bst_size_pl0,
+            C.bst_keys_pl0, C.bst_repr_pl0, C.bst_depth_pl0, C.bst_root_pl0,
+            C.next_pl0, C.prev_pl0, C.list_keys_pl0, C.list_repr_pl0,
+            root
+        );
+        invariant Unchanged(
+            C.k, C.l, C.r, C.p, C.min, C.max, C.bst_size,
+            C.bst_keys, C.bst_repr, C.bst_depth, C.bst_root,
+            C.next, C.prev, C.list_keys, C.list_repr,
+            C.k_pl0, C.l_pl0, C.r_pl0, C.p_pl0, C.min_pl0, C.max_pl0, C.bst_size_pl0,
+            C.bst_keys_pl0, C.bst_repr_pl0, C.bst_depth_pl0, C.bst_root_pl0,
+            C.next_pl0, C.prev_pl0, C.list_keys_pl0, C.list_repr_pl0,
+            node
+        );
+        invariant ret != null ==>
+            Unchanged(
+                C.k, C.l, C.r, C.p, C.min, C.max, C.bst_size,
+                C.bst_keys, C.bst_repr, C.bst_depth, C.bst_root,
+                C.next, C.prev, C.list_keys, C.list_repr,
+                C.k_pl0, C.l_pl0, C.r_pl0, C.p_pl0, C.min_pl0, C.max_pl0, C.bst_size_pl0,
+                C.bst_keys_pl0, C.bst_repr_pl0, C.bst_depth_pl0, C.bst_root_pl0,
+                C.next_pl0, C.prev_pl0, C.list_keys_pl0, C.list_repr_pl0,
+                ret
+            );
+        invariant q1s != null ==> C.bst_root[q1s] == old(C.bst_root)[q1s];
+    {
+        // Do we have a valid termination measure?
+        call t := Get_bst_depth(cur);
+        assert t >= 0;
+        z := t;
+
+        call cur_p := Get_p(cur);
+        call IfNotBr_ThenLC(cur_p);
+        call cur_l := Get_l(cur);
+        call cur_r := Get_r(cur);
+        call IfNotBr_ThenLC(cur_l);
+        call IfNotBr_ThenLC(cur_r);
+
+        call cur_k := Get_k(cur);
+        call cur_l_bst_size := GetBSTSizeOrZero(cur_l);
+        call cur_r_bst_size := GetBSTSizeOrZero(cur_r);
+        if (cur_l != null) {
+            call cur_l_min := Get_min(cur_l);
+            call cur_l_bst_keys := Get_bst_keys(cur_l);
+            call cur_l_bst_repr := Get_bst_repr(cur_l);
+        }
+        if (cur_r != null) {
+            call cur_r_max := Get_max(cur_r);
+            call cur_r_bst_keys := Get_bst_keys(cur_r);
+            call cur_r_bst_repr := Get_bst_repr(cur_r);
+        }
+        call Set_bst_size(cur, cur_l_bst_size + 1 + cur_r_bst_size);
+        call Set_bst_repr(
+            cur,
+            RefSetUnionF(
+                if cur_l == null then EmptyRefSet else cur_l_bst_repr,
+                if cur_r == null then EmptyRefSet else cur_r_bst_repr
+            )[cur := true]
+        );
+        call Set_bst_keys(
+            cur,
+            KeySetUnionF(
+                if cur_l == null then EmptyKeySet else cur_l_bst_keys,
+                if cur_r == null then EmptyKeySet else cur_r_bst_keys
+            )[cur_k := true]
+        );
+        call Set_min(cur, if cur_l == null then cur_k else cur_l_min);
+        call Set_max(cur, if cur_r == null then cur_k else cur_r_max);
+        call AssertLCAndRemove(cur);
+
+        call cur_p := Get_p(cur);
+        cur := cur_p;
+
+        call IfNotBrList_ThenListLC(cur);
+
+        call cur_p := Get_p(cur);
+
+        // Has our termination measure decreased?
+        call t := Get_bst_depth(cur);
+        assert t < z;
+    }
+
+    ret := ret;
+    ret := ret;
+    assume false;
+}
