boogie/scheduler-queue/bst-fix-depth.bpl
@@ -5,6 +5,9 @@
 // Artifact by Cody Rivera, 2023. 
 //
 // Verification of depth fixing for BSTs, for overlaid data structures.
+//
+// Since this is a ghost method, we must explicitly prove termination in
+// order for the framework to be sound.
 
 procedure BSTFixDepthContract(q1s: Ref, q1t: Ref, x: Ref);
     requires x != null;
@@ -13,22 +16,22 @@ procedure BSTFixDepthContract(q1s: Ref, q1t: Ref, x: Ref);
         Br_bst
     );
     requires RefSetsEqual(Br_list, EmptyRefSet);
-    requires LC_Trans_NoDepth(C.k, C.l, C.r, C.p, C.min, C.max,
+    requires LC_Trans_NoDepth(C.k, C.l, C.r, C.p, C.min, C.max, C.bst_size,
                 C.bst_keys, C.bst_repr, C.bst_depth, C.bst_root,
                 C.next, C.prev, C.list_keys, C.list_repr, x);
     requires C.p[x] != null;
     modifies Br_bst, Br_list, C.bst_depth;
-    ensures LC(C.k, C.l, C.r, C.p, C.min, C.max,
+    ensures LC(C.k, C.l, C.r, C.p, C.min, C.max, C.bst_size,
                 C.bst_keys, C.bst_repr, C.bst_depth, C.bst_root,
                 C.next, C.prev, C.list_keys, C.list_repr, x);
     ensures RefSetsEqual(Br_bst, old(Br_bst)[x := false]);
     ensures RefSetsEqual(Br_list, EmptyRefSet);
     // Framing conditions
     ensures Frame_all(
-        C.k, C.l, C.r, C.p, C.min, C.max,
+        C.k, C.l, C.r, C.p, C.min, C.max, C.bst_size,
         C.bst_keys, C.bst_repr, C.bst_depth, C.bst_root,
         C.next, C.prev, C.list_keys, C.list_repr,
-        old(C.k), old(C.l), old(C.r), old(C.p), old(C.min), old(C.max),
+        old(C.k), old(C.l), old(C.r), old(C.p), old(C.min), old(C.max), old(C.bst_size),
         old(C.bst_keys), old(C.bst_repr), old(C.bst_depth), old(C.bst_root),
         old(C.next), old(C.prev), old(C.list_keys), old(C.list_repr),
         RefSetIntersectF(old(C.bst_repr)[x], old(C.bst_repr)[old(C.bst_root)[x]]), old(alloc)
@@ -41,22 +44,22 @@ procedure BSTFixDepth(q1s: Ref, q1t: Ref, x: Ref)
         Br_bst
     );
     requires RefSetsEqual(Br_list, EmptyRefSet);
-    requires LC_Trans_NoDepth(C.k, C.l, C.r, C.p, C.min, C.max,
+    requires LC_Trans_NoDepth(C.k, C.l, C.r, C.p, C.min, C.max, C.bst_size,
                 C.bst_keys, C.bst_repr, C.bst_depth, C.bst_root,
                 C.next, C.prev, C.list_keys, C.list_repr, x);
     requires C.p[x] != null;
     modifies Br_bst, Br_list, C.bst_depth;
-    ensures LC(C.k, C.l, C.r, C.p, C.min, C.max,
+    ensures LC(C.k, C.l, C.r, C.p, C.min, C.max, C.bst_size,
                 C.bst_keys, C.bst_repr, C.bst_depth, C.bst_root,
                 C.next, C.prev, C.list_keys, C.list_repr, x);
     ensures RefSetsEqual(Br_bst, old(Br_bst)[x := false]);
     ensures RefSetsEqual(Br_list, EmptyRefSet);
     // Framing conditions
     ensures Frame_all(
-        C.k, C.l, C.r, C.p, C.min, C.max,
+        C.k, C.l, C.r, C.p, C.min, C.max, C.bst_size,
         C.bst_keys, C.bst_repr, C.bst_depth, C.bst_root,
         C.next, C.prev, C.list_keys, C.list_repr,
-        old(C.k), old(C.l), old(C.r), old(C.p), old(C.min), old(C.max),
+        old(C.k), old(C.l), old(C.r), old(C.p), old(C.min), old(C.max), old(C.bst_size),
         old(C.bst_keys), old(C.bst_repr), old(C.bst_depth), old(C.bst_root),
         old(C.next), old(C.prev), old(C.list_keys), old(C.list_repr),
         RefSetIntersectF(old(C.bst_repr)[x], old(C.bst_repr)[old(C.bst_root)[x]]), old(alloc)
@@ -67,6 +70,18 @@ procedure BSTFixDepth(q1s: Ref, q1t: Ref, x: Ref)
     var x_r: Ref;
     var x_p: Ref;
     var x_p_bst_depth: int;
+    var x_l_bst_size: int;
+    var x_r_bst_size: int;
+
+    // Termination measure variables.
+    var t: int;
+    var z: int;
+
+    // Do we have a valid termination measure?
+    call t := Get_bst_size(x);
+    assert t >= 0;
+    // Store termination measure.
+    z := t;
 
     call InAllocParam(q1s);
     call InAllocParam(q1t);
@@ -88,10 +103,18 @@ procedure BSTFixDepth(q1s: Ref, q1t: Ref, x: Ref)
     call x_l := Get_l(x);
     call x_r := Get_r(x);
     if (x_l != null) {
+        call x_l_bst_size := Get_bst_size(x_l);
+        t := x_l_bst_size;
+        // Does our measure decrease before our call?
+        assert t < z;
         call BSTFixDepthContract(q1s, q1t, x_l);
     }
     if (x_r != null) {
         call IfNotBrList_ThenListLC(x_r);
+        call x_r_bst_size := Get_bst_size(x_r);
+        t := x_r_bst_size;
+        // Does our measure decrease before our call?
+        assert t < z;
         call BSTFixDepthContract(q1s, q1t, x_r);
     }
     call IfNotBrList_ThenListLC(x);
